TestDuration.dfy
@@ -2,7 +2,7 @@ include "Duration.dfy"
 
 module TestDuration {
   import Std.DateTime.Duration
-
+ 
   method Main() {
     var d1 := Duration.Duration(10, 500);
     var d2 := Duration.Duration(5, 250);
@@ -30,7 +30,73 @@ module TestDuration {
     // Equality
     assert Duration.Equal(d1, d1);
     assert !Duration.Equal(d1, d2);
-  }
+
+//basic math and roundtrip correctness
+
+  var d := Duration.Duration(2, 500); // 2.5 seconds
+  var scaled := Duration.Scale(d, 2); // 5 seconds
+  assert Duration.ToTotalMilliseconds(scaled) == 5000;
+
+  var divided := Duration.Divide(scaled, 2);
+  assert Duration.Equal(divided, d);
+
+  var mod := Duration.Mod(scaled, d);
+  assert Duration.Equal(mod, Duration.FromMilliseconds(0));
+
+  var dmin := Duration.Min(d, scaled);
+  var dmax := Duration.Max(d, scaled);
+  assert Duration.Equal(dmin, d);
+  assert Duration.Equal(dmax, scaled);
+//Conversion between seconds, minutes, hours
+  var oneSec := Duration.FromSeconds(1);
+  assert Duration.ToTotalMilliseconds(oneSec) == 1000;
+
+  var oneMin := Duration.FromMinutes(1);
+  assert Duration.ToTotalMilliseconds(oneMin) == 60000;
+
+  var oneHour := Duration.FromHours(1);
+  assert Duration.ToTotalMilliseconds(oneHour) == 3600000;
+
+  var oneDay := Duration.FromDays(1);
+  assert Duration.ToTotalMilliseconds(oneDay) == 86400000;
+// Sequence Aggregation(Min/Max)
+  var d_1 := Duration.Duration(0, 500);
+  var d_2 := Duration.Duration(1, 0);
+  var d_3 := Duration.Duration(1, 500);
+
+//  var seq: seq<Duration.Duration> := [d_1, d2, d3];
+
+//  var maxD := Std.DateTime.Duration.Max(seq);
+//  var minD := Std.DateTime.Duration.Min(seq);
+
+//  assert Duration.Equal(maxD, d3);
+//  assert Duration.Equal(minD, d1);
+
+//comparing edge cases
+  var d5 := Duration.FromMilliseconds(1000);
+  var d6 := Duration.FromMilliseconds(999);
+  assert Duration.Less(d6, d5);
+  assert !Duration.Less(d5, d6);
+
+  assert Duration.Compare(d5, d5) == 0;
+  assert Duration.Compare(d5, d6) == 1;
+  assert Duration.Compare(d6, d5) == -1;
   
+// comparing epoch difference
+   var e1 := 5000;
+   var e2 := 8000;
+   var dd := Duration.EpochDifference(e1, e2);
+   assert Duration.ToTotalMilliseconds(dd) == 3000;
+
+   // Symmetry check
+   var d7 := Duration.EpochDifference(e2, e1);
+   assert Duration.Equal(d, d7);
+//normalization
+  var d8 := Duration.FromMilliseconds(2500);
+  assert Duration.GetSeconds(d8) == 2;
+  assert Duration.GetMilliseconds(d8) == 500;
+ //dafny verify TestDuration.dfy
+  }
+
 }
 
